\documentclass{article}
\usepackage[utf8]{inputenc}
\usepackage{amsmath}

\begin{document}

\section{The sequence of even numbers}
The generating function of the sequence of even numbers $\langle 0, 2, 4, 6, \cdots \rangle$ \ is\\
$${f_1(x)} = {\sum_{n \geq 0} x^{2n}}$$

\begin{align*}
    f_1(x) \cdot x^2 + x^0 & = \sum_{n \geq 0} x^{2(n + 1)} + x^0 \\
                           & = \sum_{n \geq 1} x^{2n} + x^0       \\
                           & = f_1(x)                             \\
\end{align*}

\begin{align*}
    f_1(x) \cdot (x^2 - 1) = -1 \\
    f_1(x) = \frac{1}{1 - x^2}
\end{align*}

\section{The sequence of 0 and 1}
The generating function of the sequence of 0 and 1 $\langle 0, 1 \rangle$ \ is\\
$$f_2(x) = \sum_{n \in \{0, 1\}} x^n$$

\begin{align*}
    f_2(x) & = x^0 + x^1 \\
           & = 1 + x
\end{align*}

\section{The sequence of 0, 1 and 2}
The generating function of the sequence of 0, 1 and 2 $\langle 0, 1, 2 \rangle$ \ is\\
$$f_3(x) = \sum_{n \in \{0, 1, 2\}} x^n$$

\begin{align*}
    f_3(x) & = x^0 + x^1 + x^2 \\
           & = 1 + x + x^2
\end{align*}

\section{The sequence of odd numbers}
The generating function of the sequence of odd numbers $\langle 1, 3, 5, 7, \cdots \rangle$ \ is\\
$${f_4(x)} = {\sum_{n \geq 0} x^{2n + 1}}$$

\begin{align*}
    f_4(x) \cdot x^2 + x & = \sum_{n \geq 0} x^{2(n + 1) + 1} + x \\
                         & = \sum_{n \geq 1} x^{2n + 1} + x       \\
                         & = f_4(x)
\end{align*}

\begin{align*}
    f_4(x) \cdot (x^2 - 1) = -x \\
    f_4(x) = \frac{x}{1 - x^2}
\end{align*}

\section{The sequence of multiples of 4}
The generating function of the sequence of multiples of 4 $\langle 0, 4, 8, 12, \cdots \rangle$ \ is\\
$${f_5(x)} = {\sum_{n \geq 0} x^{4n}}$$

\begin{align*}
    f_5(x) \cdot x^4 + x^0 & = \sum_{n \geq 0} x^{4(n + 1)} + x^0 \\
                           & = \sum_{n \geq 1} x^{4n} + x^0       \\
                           & = f_5(x)
\end{align*}

\begin{align*}
    f_5(x) \cdot (x^4 - 1) = -1 \\
    f_5(x) = \frac{1}{1 - x^4}
\end{align*}

\section{The sequence of 0, 1, 2 and 3}
The generating function of the sequence of 0, 1, 2 and 3 $\langle 0, 1, 2, 3 \rangle$ \ is\\
$$f_6(x) = \sum_{n \in \{0, 1, 2, 3\}} x^n$$

\begin{align*}
    f_6(x) & = x^0 + x^1 + x^2 + x^3 \\
           & = 1 + x + x^2 + x^3     \\
           & = (x + 1)(x^2 + 1)
\end{align*}

\section{The sequence of multiples of 3}
The generating function of the sequence of multiples of 3 $\langle 0, 3, 6, 9, \cdots \rangle$ \ is\\
$${f_7(x)} = {\sum_{n \geq 0} x^{3n}}$$

\begin{align*}
    f_7(x) \cdot x^3 + x^0 & = \sum_{n \geq 0} x^{3(n + 1)} + x^0 \\
                           & = \sum_{n \geq 1} x^{3n} + x^0       \\
                           & = f_7(x)
\end{align*}

\begin{align*}
    f_7(x) \cdot (x^3 - 1) = -1 \\
    f_7(x) = \frac{1}{1 - x^3}
\end{align*}

\end{document}
